reflection_example.v
@@ -1,0 +1,29 @@
+Local Open Scope bool.
+
+Lemma reduce_prop:
+  forall (P Q R :Prop),
+  Q -> R -> ~P ->
+    (Q \/ ~R) /\ (P \/ (~P /\ R /\ Q)).
+Proof.
+  intros.
+  split.
+    (* Q \/ ~R *)
+    left. assumption.
+    (* P /\ (~P /\ R /\ Q) *)
+    right. 
+    split.
+      (* ~ P *) assumption.
+    split.
+      (* R *) assumption.
+      (* Q *) assumption.
+Qed.
+
+Lemma reduce_bool:
+  forall (p q r :bool),
+  q = true -> r = true -> p = false ->
+    (q || (negb r)) && (p || ((negb p) && r && q)) = true.
+Proof.
+  intros. rewrite H. rewrite H0. rewrite H1.
+  compute.
+  reflexivity.
+Qed.
